Remove one source of tuple allocations
make -C src/Parsers/Refinement/Testing
make[1]: Entering directory '/cygdrive/d/Documents/GitHub/fiat/src/Parsers/Refinement/Testing'
make -f Makefile.ab_star test-pretty
make[2]: Entering directory '/cygdrive/d/Documents/GitHub/fiat/src/Parsers/Refinement/Testing'
make -f Makefile.ab_star test 2>&1 | python format-test-output.py
reference (10        ): total: 0.000000, median: 0.000000, mean: 0.000000, sample variance: 0.000000, iterations: 10 (10 on each)
coq       (10        ): total: 0.000000, median: 0.000000, mean: 0.000000, sample variance: 0.000000, iterations: 10 (10 on each)
reference (100       ): total: 0.000000, median: 0.000000, mean: 0.000000, sample variance: 0.000000, iterations: 10 (10 on each)
coq       (100       ): total: 0.001000, median: 0.000000, mean: 0.000100, sample variance: 0.000000, iterations: 10 (10 on each)
reference (1000      ): total: 0.000000, median: 0.000000, mean: 0.000000, sample variance: 0.000000, iterations: 10 (10 on each)
coq       (1000      ): total: 0.015000, median: 0.001500, mean: 0.001500, sample variance: 0.000000, iterations: 10 (10 on each)
reference (10000     ): total: 0.006000, median: 0.001000, mean: 0.000600, sample variance: 0.000000, iterations: 10 (10 on each)
coq       (10000     ): total: 0.167000, median: 0.016000, mean: 0.016700, sample variance: 0.000003, iterations: 10 (10 on each)
reference (100000    ): total: 0.055000, median: 0.005500, mean: 0.005500, sample variance: 0.000000, iterations: 10 (10 on each)
coq       (100000    ): total: 2.703000, median: 0.271500, mean: 0.270300, sample variance: 0.000171, iterations: 10 (10 on each)
reference (1000000   ): total: 0.572000, median: 0.056000, mean: 0.057200, sample variance: 0.000021, iterations: 10 (10 on each)
-------------------------------------------------
          10 |   0.000000 s |  0.000000 s |   N/A
         100 |   0.000000 s |  0.000000 s |   N/A
        1000 |   0.000000 s |  0.000150 s |   N/A
       10000 |   0.000100 s |  0.001600 s | 1600.0 % slower
      100000 |   0.000550 s |  0.027150 s | 4936.36363636 % slower
     1000000 |   0.005600 s |        None |   N/A
make[2]: Leaving directory '/cygdrive/d/Documents/GitHub/fiat/src/Parsers/Refinement/Testing'
make[1]: Leaving directory '/cygdrive/d/Documents/GitHub/fiat/src/Parsers/Refinement/Testing'

src/Parsers/BooleanRecognizerOptimized.v
@@ -4,7 +4,7 @@ Require Import Coq.Numbers.Natural.Peano.NPeano Coq.Arith.Compare_dec Coq.Arith.
 Require Import Fiat.Parsers.ContextFreeGrammar.Core.
 Require Import Fiat.Parsers.ContextFreeGrammar.Notations.
 Require Import Fiat.Parsers.BaseTypes.
-Require Import Fiat.Common Fiat.Common.Wf.
+Require Import Fiat.Common Fiat.Common.Wf Fiat.Common.Wf2 Fiat.Common.Telescope.Core.
 Require Import Fiat.Parsers.BooleanRecognizer.
 Require Import Fiat.Parsers.BooleanRecognizerCorrect.
 Require Import Fiat.Parsers.BooleanRecognizerExt.
@@ -268,16 +268,16 @@ Section recursive_descent_parser.
     { apply IH; t_reduce_fix. }
   Defined.
 
-  Local Ltac refine_Fix5_Proper_eq :=
+  Local Ltac refine_Fix2_5_Proper_eq :=
     idtac;
     (lazymatch goal with
-    | [ |- context[_ = @Fix ?A ?R ?Rwf ?T (fun a0 b0 c0 d0 e0 h0 i0 => @?f a0 b0 c0 d0 e0 h0 i0) ?a ?b ?c ?d ?e ?h] ]
+    | [ |- context[_ = @Fix2 ?A ?A' ?R ?Rwf ?T (fun a0 b0 c0 d0 e0 h0 i0 => @?f a0 b0 c0 d0 e0 h0 i0) ?a ?a' ?b ?c ?d ?e ?h] ]
       => (lazymatch T with
-         | (fun a' : ?A => forall (b' :@?B a') (c' : @?C a' b') (d' : @?D a' b' c') (e' : @?E a' b' c' d') (h' : @?H a' b' c' d' e'), @?P a' b' c' d' e' h')
+         | (fun a' : ?A0 => forall (b' :@?B a') (c' : @?C a' b') (d' : @?D a' b' c') (e' : @?E a' b' c' d') (h' : @?H a' b' c' d' e'), @?P a' b' c' d' e' h')
            => let H' := fresh in
               (*refine (_ : @Fix A R Rwf T (fun a0 b0 c0 d0 e0 h0 i0 => _) a b c d e h = _);
                  let f' := match goal with |- @Fix _ _ _ _ ?f' _ _ _ _ _ _ = _ => constr:f' end in*)
-              pose proof ((fun f' H0 => @Fix5_Proper_eq A B C D E H R Rwf P f' f H0 a b c d e h)) as H';
+              pose proof ((fun f' H0 => @Fix2_5_Proper_eq A A' B C D E H R Rwf P f' f H0 a a' b c d e h)) as H';
           cbv beta in H';
           (lazymatch type of H' with
           | forall f' : ?f'T, @?H'T f' -> _
@@ -361,9 +361,9 @@ Section recursive_descent_parser.
       | _ => constr:RHS
     end.
 
-  Local Ltac fix_trans :=
+  Local Ltac fix2_trans :=
     match goal with
-      | [ H : forall a0 a1 a2 a3 a4 a5 a6, ?x a0 a1 a2 a3 a4 a5 a6 = ?y a0 a1 a2 a3 a4 a5 a6 |- _ = ?RHS ]
+      | [ H : forall a0 a0' a1 a2 a3 a4 a5 a6, ?x a0 a0' a1 a2 a3 a4 a5 a6 = ?y a0 a0' a1 a2 a3 a4 a5 a6 |- _ = ?RHS ]
         => let RHS' := fix_trans_helper RHS x y
            in transitivity RHS'; [ clear H y | ]
     end.
@@ -378,7 +378,7 @@ Section recursive_descent_parser.
           t_reduce_list)
      end).
 
-  Definition parse_nonterminal_opt'
+  Definition parse_nonterminal_opt'0
              (str : String)
              (nt : String.string)
   : { b : bool | b = parse_nonterminal (G := G) str nt }.
@@ -390,12 +390,25 @@ Section recursive_descent_parser.
     let G := match goal with |- context[_ = parse_nonterminal (G := ?G) _ _] => constr:G end in
     let G' := head G in
     unfold G'.
+    cbv beta iota zeta delta [parse_nonterminal parse_nonterminal_or_abort list_to_grammar].
+    change (@parse_nonterminal_step) with (fun a b c d e f g h i j k l => @parse_nonterminal_step a b c d e f g h i j k l); cbv beta.
+    evar (b : bool).
+    sigL_transitivity b; subst b;
+    [
+    | rewrite Fix5_2_5_eq by (intros; apply parse_nonterminal_step_ext; assumption);
+      reflexivity ].
+    simpl @fst; simpl @snd.
     cbv beta iota zeta delta [parse_nonterminal parse_nonterminal_or_abort parse_nonterminal_step parse_productions parse_productions' parse_production parse_item parse_item' Lookup list_to_grammar list_to_productions].
     simpl.
     cbv beta iota zeta delta [rdp_list_nonterminals_listT rdp_list_is_valid_nonterminal rdp_list_remove_nonterminal].
-    refine_Fix5_Proper_eq.
+    evar (b : bool).
+    sigL_transitivity b; subst b;
+    [
+    | rewrite <- !surjective_pairing, !to_of;
+      reflexivity ].
+    refine_Fix2_5_Proper_eq.
     unfold parse_production', parse_production'_for, parse_item'.
-    fix_trans;
+    fix2_trans;
       [
       | solve [ t_reduce_fix;
                 t_reduce_list_more;
@@ -476,26 +489,12 @@ Section recursive_descent_parser.
     reflexivity.
   Defined.
 
-  Definition parse_nonterminal_opt''
-             (str : String)
-             (nt : String.string)
-  : { b : bool | b = parse_nonterminal (G := G) str nt }.
-  Proof.
-    let c := constr:(parse_nonterminal_opt' str nt) in
-    let h := head c in
-    let p := (eval cbv beta iota zeta delta [proj1_sig h] in (proj1_sig c)) in
-    sigL_transitivity p; [ | abstract exact (proj2_sig c) ].
-    eexists.
-    rewrite <- !surjective_pairing, !to_of.
-    reflexivity.
-  Defined.
-
   Definition parse_nonterminal_opt
              (str : String)
              (nt : String.string)
   : { b : bool | b = parse_nonterminal (G := G) str nt }.
   Proof.
-    let c := constr:(parse_nonterminal_opt'' str nt) in
+    let c := constr:(parse_nonterminal_opt'0 str nt) in
     let h := head c in
     let impl := (eval cbv beta iota zeta delta [h proj1_sig] in (proj1_sig c)) in
     (exists impl);
